port all the base rules to be about wp, pvs only

iris_core.v
@@ -424,6 +424,9 @@ Module Type IRIS_CORE (RL : RA_T) (C : CORE_LANG) (R: IRIS_RES RL C) (WP: WORLD_
     - intros w n r; apply Hp; exact I.
   Qed.
 
+  (* People will need that *)
+  Definition wf_nat_ind := well_founded_induction Wf_nat.lt_wf.
+
 End IRIS_CORE.
 
 Module IrisCore (RL : RA_T) (C : CORE_LANG) (R: IRIS_RES RL C) (WP: WORLD_PROP R) : IRIS_CORE RL C R WP.
